defining memory system incl instruction cache, first lemmas

msIfScript.sml
@@ -6,7 +6,7 @@ open wordsLib blastLib;
 open basetypesTheory;
 open cachememTheory;
 
-val _ = new_theory "coreIf";
+val _ = new_theory "msIf";
 
 (* TODO: 
 - ms record type
@@ -15,6 +15,118 @@ val _ = new_theory "coreIf";
 - lift deriveability lemmas
 - IC lemmas / invariant
 *)
+
+val _ = Datatype `memsys_state = <| 
+    dc  : cache_state;
+    ic  : cache_state;
+    mem : mem_state 
+|>`;
+
+val dw_def = Define `dw ms pa = ms.dc pa`;
+val dhit_def = Define `dhit ms pa = chit_ ms.dc pa`;
+val dirty_def = Define `dirty ms pa = cdirty_ ms.dc pa`;
+val dcnt_def = Define `dcnt ms pa = ccnt_ ms.dc pa`;
+val M_def = Define `M ms pa = ms.mem pa`;
+
+val iw_def = Define `iw ms pa = ms.ic pa`;
+val ihit_def = Define `ihit ms pa = chit_ ms.ic pa`;
+val icnt_def = Define `icnt ms pa = ccnt_ ms.ic pa`;
+
+(* instruction cache invariant *)
+
+val Invic_def = Define `Invic ms = !pa. ~cdirty_ ms.ic pa`;
+
+(* lookup functions / memory views *)
+
+val dmvcl_def = Define `dmvcl ms = MVcl ms.mem`;
+val dmvca_def = Define `dmvca ms = MVca ms.dc ms.mem`;
+val dmvalt_def = Define `dmvalt ms = MValt ms.dc ms.mem`;
+val imv_def = Define `imv ms = MVca ms.ic ms.mem`;
+
+(* transition system *)
+
+val ms_dupd_def = Define `
+ms_dupd ms (ca,m) = ms with <| dc := ca; mem := m |>
+`;
+
+val ms_dupd_rw = store_thm("ms_dupd_rw", ``
+!ms ca m. ((ms_dupd ms (ca,m)).dc = ca)
+       /\ ((ms_dupd ms (ca,m)).ic = ms.ic)
+       /\ ((ms_dupd ms (ca,m)).mem = m)
+``,
+  RW_TAC std_ss [ms_dupd_def]
+);
+
+val ms_iupd_def = Define `
+ms_iupd ms (ca,m) = ms with <| ic := ca |>
+`;
+
+val ms_iupd_rw = store_thm("ms_iupd_rw", ``
+!ms ca m. ((ms_iupd ms (ca,m)).dc = ms.dc)
+       /\ ((ms_iupd ms (ca,m)).ic = ca)
+       /\ ((ms_iupd ms (ca,m)).mem = ms.mem)
+``,
+  RW_TAC std_ss [ms_iupd_def]
+);
+
+val ms_mupd_def = Define `
+ms_mupd ms m = ms with <| mem := m |>
+`;
+
+val ms_mupd_rw = store_thm("ms_mupd_rw", ``
+!ms ca m. ((ms_mupd ms m).dc = ms.dc)
+       /\ ((ms_mupd ms m).ic = ms.ic)
+       /\ ((ms_mupd ms m).mem = m)
+``,
+  RW_TAC std_ss [ms_mupd_def]
+);
+
+val msca_trans_def = Define `
+   (msca_trans ms (DREQ dop) = ms_dupd ms (mtfca (ms.dc, ms.mem) dop))
+/\ (msca_trans ms (FREQ pa) = ms_iupd ms (mtfca (ms.ic, ms.mem) (RD pa T)))
+/\ (msca_trans ms NOREQ = ms)
+`;
+
+val mtf_pat = ``(x,y) = mtfca (a,b) c``; 
+
+val mtf_pat2 = ``mtfca (a,b) c = (x,y)``; 
+
+fun ASM_SYM_TAC pat = PAT_X_ASSUM pat (fn thm => ASSUME_TAC (SYM thm));
+
+
+val msca_DREQ_lem = store_thm("msca_DREQ_lem", ``
+!ms dop ms'. (ms' = msca_trans ms (DREQ dop)) 
+    ==>
+?ca' m'. ((ca',m') = mtfca (ms.dc, ms.mem) dop) 
+      /\ (ms'.dc = ca')
+      /\ (ms'.ic = ms.ic)
+      /\ (ms'.mem = m')
+``,
+  REWRITE_TAC [msca_trans_def] >> 
+  REPEAT STRIP_TAC >>
+  `?ca' m'. (ca',m') = mtfca (ms.dc, ms.mem) dop` by (
+      METIS_TAC [pairTheory.pair_CASES]
+  ) >>
+  EXISTS_TAC ``ca':cache_state`` >>
+  EXISTS_TAC ``m':mem_state`` >>
+  ASM_SYM_TAC mtf_pat >>
+  ASM_REWRITE_TAC [ms_dupd_rw]
+);
+
+(* deriveability obligations *)
+
+val ms_cacheable_other_oblg = store_thm("ms_cacheable_other_oblg", ``
+!ms dop ms' pa. CA dop /\ (ms' = msca_trans ms (DREQ dop)) /\ (pa <> PA dop)
+             /\ (dw ms' pa <> dw ms pa) ==> 
+    ~dhit ms' pa
+``,
+  REPEAT GEN_TAC >>
+  STRIP_TAC >>
+  IMP_RES_TAC msca_DREQ_lem >>
+  FULL_SIMP_TAC std_ss [dw_def, dhit_def] >>
+  IMP_RES_TAC ca_cacheable_other_lem
+);
+
 
 (*********** finish ************)
 
